theories/lang/cpp/semantics/values.v
@@ -20,13 +20,45 @@ Require Import bedrock.lang.cpp.semantics.sub_module.
 
 Set Default Proof Using "Type".
 
-(** pointers *)
+(** * pointers
+    this is the abstract model of pointers in C++.
+    - A simple model is [block * offset] which is representing a collection
+      of isolated blocks. There is no address arithmetic that can get you
+      from one block to another.
+    - A more complex model allows for nested blocks and more accurately
+      models the C/C++ (object) memory model. See
+      https://robbertkrebbers.nl/thesis.html
+ *)
 Parameter ptr : Set.
 Parameter ptr_eq_dec : forall (x y : ptr), { x = y } + { x <> y }.
+Instance: EqDecision ptr := ptr_eq_dec.
+Instance: Countable ptr.
+Proof. Admitted.
+
+(** C++ provides a distinguished pointer [nullptr] that is *never
+    dereferenable*
+ *)
 Parameter nullptr : ptr.
 
 
-(** values *)
+(** ** pointer offsets *)
+(** the offset of a pointer. *)
+Parameter offset_ptr_ : Z -> ptr -> ptr.
+
+Axiom offset_ptr_combine_ : forall b o o',
+    offset_ptr_ o' (offset_ptr_ o b) = offset_ptr_ (o + o') b.
+Axiom offset_ptr_0_ : forall b,
+    offset_ptr_ 0 b = b.
+
+
+(** * values
+    abstract C++ runtime values come in two flavors.
+    - integers
+    - pointers
+    there is also a distinguished undefined element [Vundef] that
+    models uninitialized values. Operations on [Vundef] are all
+    undefined behavior.
+ *)
 Variant val : Set :=
 | Vint (_ : Z)
 | Vptr (_ : ptr)
@@ -37,7 +69,9 @@ Definition val_dec : forall a b : val, {a = b} + {a <> b}.
 Proof.
   decide equality. eapply Z.eq_dec. apply ptr_eq_dec.
 Defined.
+Instance: EqDecision val := val_dec.
 
+(** wrappers for constructing certain values *)
 Definition Vchar (a : Ascii.ascii) : val :=
   Vint (Z.of_N (N_of_ascii a)).
 Definition Vbool (b : bool) : val :=
@@ -47,7 +81,20 @@ Definition Vnat (b : nat) : val :=
 Definition Vn (b : N) : val :=
   Vint (Z.of_N b).
 Notation Vz := Vint (only parsing).
+
+(** we use [Vundef] as our value of type [void] *)
 Definition Vvoid := Vundef.
+
+(** lifting pointer offsets to values *)
+Definition offset_ptr (o : Z) (v : val) : val :=
+  match v with
+  | Vptr p => Vptr (offset_ptr_ o p)
+  | _ => Vundef
+  end.
+Theorem offset_ptr_val : forall v o p,
+    Vptr p = v ->
+    Vptr (offset_ptr_ o p) = offset_ptr o v.
+Proof. intros; subst; reflexivity. Qed.
 
 Definition is_true (v : val) : option bool :=
   match v with
@@ -68,55 +115,57 @@ Proof. inversion 1; reflexivity. Qed.
 Theorem Vint_inj : forall a b, Vint a = Vint b -> a = b.
 Proof. inversion 1; reflexivity. Qed.
 
-(* this is the stack frame *)
-Parameter region : Type.
+(** * regions
+    to model the stack frame in separation logic, we use a notion of regions
+    that are threaded through the semantics.
 
-(** pointer offsets *)
-(* All offsets are valid pointers. todo: This is unsound. *)
-Parameter offset_ptr_ : Z -> ptr -> ptr.
+    here, we instantiate [region] as [ptr] which allows us to extend regions
+    at runtime (when new variables are declared).
 
-Axiom offset_ptr_combine_ : forall b o o',
-    offset_ptr_ o' (offset_ptr_ o b) = offset_ptr_ (o + o') b.
-Axiom offset_ptr_0_ : forall b,
-    offset_ptr_ 0 b = b.
-
-
-Parameter offset_ptr : Z -> val -> val.
-(* note(gmm): this is not defined according to the C semantics because creating
- * a pointer that goes out of bounds of the object is undefined behavior in C,
- * e.g. [(p + a) - a <> p] if [p + a] is out of bounds.
+    an alternative model is to instantiate region as [gmap ident ptr]
+    essentially giving a location to each local variable.
+    todo: change to this model?
  *)
-Axiom offset_ptr_combine : forall b o o',
-    offset_ptr o' (offset_ptr o b) = offset_ptr (o + o') b.
-Axiom offset_ptr_0 : forall b,
-    offset_ptr 0 b = b.
-Axiom offset_ptr_val : forall v o p, Vptr p = v -> Vptr (offset_ptr_ o p) = offset_ptr o v.
+Definition region : Type := ptr.
 
+(** * global environments *)
 
-(** global environments *)
+(** this contains two things:
+   - the types declared in the program
+   - the program's symbol table (mapping of globals to pointers)
+     (this is not necessarily the same as a the symbol table in the
+      object file because it will contain the addresses of [static]
+      variables)
 
-(* this contains two things:
- * - the types declared in the program
- * - the program's symbol table (mapping of globals to pointers)
- *   (this is not necessarily the same as a the symbol table in the
- *    object file because it will contain the addresses of [static]
- *    variables)
- *
- * if we want to do things like word-size agnostic verification, then
- * information like that would need to be in here as well.
+   if we want to do things like word-size agnostic verification, then
+   information like that would need to be in here as well.
  *)
 Record genv : Type :=
 { genv_cu : compilation_unit
   (* ^ the [compilation_unit] *)
 ; glob_addr : obj_name -> option ptr
   (* ^ the address of global variables & functions *)
+; pointer_size : N
+  (* ^ the size of a pointer (in bytes) *)
 }.
 
-(* [genv_leq a b] states that [b] is an extension of [a] *)
-Parameter genv_leq : genv -> genv -> Prop.
-Global Declare Instance PreOrder_genv_leq : PreOrder genv_leq.
+(** [genv_leq a b] states that [b] is an extension of [a] *)
+Definition genv_leq (l r : genv) : Prop :=
+  sub_module l.(genv_cu) r.(genv_cu) /\
+  (forall a p, l.(glob_addr) a = Some p ->
+          r.(glob_addr) a = Some p) /\
+  l.(pointer_size) = r.(pointer_size).
+
+Instance PreOrder_genv_leq : PreOrder genv_leq.
+Proof.
+  constructor.
+  { constructor; [ | constructor ]; auto; reflexivity. }
+  { red. unfold genv_leq.
+    intros ? ? ? [A [B C]] [A' [B' C']].
+    split; [ | split ]; etransitivity; eauto. }
+Qed.
 Definition glob_def (g : genv) (gn : globname) : option GlobDecl :=
-  g.(genv_cu) !! gn.
+  g.(genv_cu).(globals) !! gn.
 
 Definition genv_eq (l r : genv) : Prop :=
   genv_leq l r /\ genv_leq r l.
@@ -131,7 +180,10 @@ Infix "⊧" := genv_compat (at level 1).
 
 Parameter subModuleModels : forall a b σ, b ⊧ σ -> module_le a b = true -> a ⊧ σ.
 
-(* todo(gmm): this should be indexed by [genv] *)
+(** typedness of values
+    note that only primitives fit into this, there is no [val] representation
+    of aggregates.
+ *)
 Parameter has_type : val -> type -> Prop.
 Arguments has_type _%Z _.
 
@@ -147,7 +199,7 @@ Definition max_val (bits : size) (sgn : signed) : Z :=
   | W64  , Unsigned => 2^64 - 1
   | W128 , Signed   => 2^127 - 1
   | W128 , Unsigned => 2^128 - 1
-  end%Z.
+  end.
 
 Definition min_val (bits : size) (sgn : signed) : Z :=
   match sgn with
@@ -160,19 +212,12 @@ Definition min_val (bits : size) (sgn : signed) : Z :=
     | W64  => -2^63
     | W128 => -2^127
     end
-  end%Z.
-
-Axiom has_type_pointer : forall v ty, has_type v (Tpointer ty) -> exists p, v = Vptr p.
+  end.
 
 Definition bound (bits : size) (sgn : signed) (v : Z) : Prop :=
   (min_val bits sgn <= v <= max_val bits sgn)%Z.
 
-Arguments Z.add _ _ : simpl never.
-Arguments Z.sub _ _ : simpl never.
-Arguments Z.mul _ _ : simpl never.
-Arguments Z.pow _ _ : simpl never.
-Arguments Z.opp _ : simpl never.
-Arguments Z.pow_pos _ _ : simpl never.
+Axiom has_type_pointer : forall v ty, has_type v (Tpointer ty) -> exists p, v = Vptr p.
 
 Axiom has_int_type : forall sz (sgn : signed) z,
     bound sz sgn z <-> has_type (Vint z) (Tint sz sgn).
@@ -195,11 +240,15 @@ Fixpoint find_field {T} (f : ident) (fs : list (ident * T)) : option T :=
     else find_field f fs
   end%list.
 
-(* todo(gmm): this isn't sound due to reference fields *)
+(* note: we expose the fact that reference fields are compiled to pointers,
+   so the [offset_of] a referene field is the offset of the pointer.
+ *)
 Definition offset_of (resolve : genv) (t : globname) (f : ident) : option Z :=
   match glob_def resolve t with
-  | Some (Gstruct s) => find_field f (List.map (fun '(a,_,c) => (a,c.(li_offset) / 8)%Z) s.(s_fields))
-  | Some (Gunion u) => find_field f (List.map (fun '(a,_,c) => (a,c.(li_offset) / 8))%Z u.(u_fields))
+  | Some (Gstruct s) =>
+    find_field f (List.map (fun '(a,_,c) => (a,c.(li_offset) / 8)%Z) s.(s_fields))
+  | Some (Gunion u) =>
+    find_field f (List.map (fun '(a,_,c) => (a,c.(li_offset) / 8))%Z u.(u_fields))
   | _ => None
   end.
 
@@ -209,52 +258,105 @@ Definition parent_offset (resolve : genv) (t : globname) (f : globname) : option
   | _ => None
   end.
 
-Parameter pointer_size : genv -> N. (* in bytes *)
-
 Variant Roption_leq {T} (R : T -> T -> Prop) : option T -> option T -> Prop :=
 | Rleq_None {x} : Roption_leq R None x
 | Rleq_Some {x y} (_ : R x y) : Roption_leq R (Some x) (Some y).
 
-(* sizeof() *)
-(* [size_of] requires a well-founded type environment in order to be
- * implementable as a function.
+(** * sizeof() *)
+(** this is a partial implementation of [size_of], it doesn't indirect through
+    typedefs, but the cpp2v generator flattens these for us anyways.
  *)
-Parameter size_of : forall (resolve : genv) (t : type), option N.
-Global Declare Instance Proper_size_of
+Fixpoint size_of (resolve : genv) (t : type) : option N :=
+  match t with
+  | Tpointer _ => Some (@pointer_size resolve)
+  | Treference _ => None
+  | Trv_reference _ => None
+  | Tint sz _ => Some (N_of_size sz)
+  | Tchar sz _ => Some (N_of_size sz)
+  | Tvoid => None
+  | Tarray t n => match size_of resolve t with
+                 | None => None
+                 | Some s => Some (n * s)
+                 end
+  | Tnamed nm =>
+    match glob_def resolve nm with
+    | Some (Gstruct s) => Some s.(s_size)
+    | Some (Gunion u) => Some u.(u_size)
+    | _ => None
+    end
+  | Tfunction _ _ => None
+  | Tbool => Some 1
+  | Tmember_pointer _ _ => Some (@pointer_size resolve)
+  | Tqualified _ t => size_of resolve t
+  | Tnullptr => Some (@pointer_size resolve)
+  | Tfloat sz => Some (N_of_size sz)
+  | Tarch sz _ => match sz with
+                 | None => None
+                 | Some sz => Some (N_of_size sz)
+                 end
+  end%N.
+
+Global Instance Proper_size_of
 : Proper (genv_leq ==> eq ==> Roption_leq eq) (@size_of).
+Proof.
+  red. red. red. intros; subst.
+  induction y0; simpl; try constructor; eauto.
+  - apply H.
+  - destruct IHy0; try constructor. subst. auto.
+  - destruct H as [ [ H _ ] _ ].
+    specialize (H g).
+    unfold glob_def, globals, Lookup_instance_0 in *.
+    destruct (globals (genv_cu x) !! g); try constructor.
+    destruct (H _ eq_refl) as [ ? [ -> HH ] ]; clear H.
+    destruct g0; try constructor;
+    destruct x0; try constructor; simpl in HH ; try congruence.
+    + apply require_eq_success in HH. destruct HH. congruence.
+    + apply require_eq_success in HH. destruct HH. congruence.
+  - apply H.
+  - apply H.
+  - destruct o; repeat constructor.
+Qed.
 
 (* it is hard to define [size_of] as a function because it needs
 to recurse through the environment in the case of [Treference]:
 termination will require a proof of well-foundedness of the environment *)
-Axiom size_of_int : forall {c : genv} s w,
-    @size_of c (Tint w s) = Some (N.div (N_of_size w + 7) 8).
-Axiom size_of_char : forall {c : genv} s w,
-    @size_of c (Tchar w s) = Some (N.div (N_of_size w + 7) 8).
-Axiom size_of_bool : forall {c : genv},
+Theorem size_of_int : forall {c : genv} s w,
+    @size_of c (Tint w s) = Some (N_of_size w).
+Proof. reflexivity. Qed.
+Theorem size_of_char : forall {c : genv} s w,
+    @size_of c (Tchar w s) = Some (N_of_size w).
+Proof. reflexivity. Qed.
+Theorem size_of_bool : forall {c : genv},
     @size_of c Tbool = Some 1%N.
-Axiom size_of_pointer : forall {c : genv} t,
+Proof. reflexivity. Qed.
+Theorem size_of_pointer : forall {c : genv} t,
     @size_of c (Tpointer t) = Some (pointer_size c).
-Axiom size_of_qualified : forall {c : genv} t q,
+Proof. reflexivity. Qed.
+Theorem size_of_qualified : forall {c : genv} t q,
     @size_of c t = @size_of c (Tqualified q t).
-Axiom size_of_array : forall {c : genv} t n sz,
+Proof. reflexivity. Qed.
+Theorem size_of_array : forall {c : genv} t n sz,
     @size_of c t = Some sz ->
-    @size_of c (Tarray t n) = Some (sz * n)%N.
+    @size_of c (Tarray t n) = Some (n * sz)%N.
+Proof. simpl; intros. rewrite H. reflexivity. Qed.
 
 Lemma size_of_Qmut : forall {c} t,
     @size_of c t = @size_of c (Qmut t).
-Proof.
-  intros.
-  now apply size_of_qualified.
-Qed.
+Proof. reflexivity. Qed.
 
 Lemma size_of_Qconst : forall {c} t ,
     @size_of c t = @size_of c (Qconst t).
-Proof.
-  intros.
-  now apply size_of_qualified.
-Qed.
+Proof. reflexivity. Qed.
 
-(* alignof() *)
+(** * alignof() *)
+(* todo: we should embed alignment information in our types *)
 Parameter align_of : forall {resolve : genv} (t : type), option N.
 Global Declare Instance Proper_align_of
 : Proper (genv_leq ==> eq ==> Roption_leq eq) (@align_of).
+
+Arguments Z.add _ _ : simpl never.
+Arguments Z.sub _ _ : simpl never.
+Arguments Z.mul _ _ : simpl never.
+Arguments Z.pow _ _ : simpl never.
+Arguments Z.opp _ : simpl never.
+Arguments Z.pow_pos _ _ : simpl never.
