theories/lang/cpp/compile.v
@@ -25,22 +25,22 @@ Section with_Σ.
       compiled code ([fspec]).
    *)
   Axiom code_at_ok : forall (f : Func) p,
-      code_at (σ:=σ) f p
+      code_at f p
       |-- Forall ti ls Q, wp_func (resolve:=σ) f ti ls Q -*
                           fspec ti (Vptr p) ls Q.
 
   Axiom method_at_ok : forall (m : Method) p,
-      method_at (σ:=σ) m p
+      method_at m p
       |-- Forall ti ls Q, wp_method (resolve:=σ) m ti ls Q -*
                           fspec ti (Vptr p) ls Q.
 
   Axiom ctor_at_ok : forall (c : Ctor) p,
-      ctor_at (σ:=σ) c p
+      ctor_at c p
       |-- Forall ti ls Q, wp_ctor (resolve:=σ) c ti ls Q -*
                           fspec ti (Vptr p) ls Q.
 
   Axiom dtor_at_ok : forall (d : Dtor) p,
-      dtor_at (σ:=σ) d p
+      dtor_at d p
       |-- Forall ti ls Q, wp_dtor (resolve:=σ) d ti ls Q -*
                           fspec ti (Vptr p) ls Q.
 
