theories/lang/cpp/logic/simple_pred.v
@@ -1,0 +1,533 @@
+(*
+ * Copyright (C) BedRock Systems Inc. 2020 Gregory Malecha
+ *
+ * SPDX-License-Identifier:AGPL-3.0-or-later
+ *)
+From iris.base_logic.lib Require Export iprop.
+From iris.bi.lib Require Import fractional.
+Require Import iris.bi.monpred.
+Require Import iris.base_logic.lib.fancy_updates.
+Require Import iris.base_logic.lib.own.
+Require Import iris.base_logic.lib.cancelable_invariants.
+Require Import iris.algebra.lib.frac_auth.
+Require Import iris.algebra.excl.
+Require Import iris.algebra.gmap.
+Require Import iris.proofmode.tactics.
+
+From bedrock.lang.cpp Require Import ast semantics.
+Require Import bedrock.lang.cpp.logic.pred.
+
+Set Default Proof Using "Type".
+
+(* todo: does this not exist as a library somewhere? *)
+Definition fractionalR (o : ofeT) : cmraT :=
+  prodR fracR (agreeR o).
+Definition frac {o: ofeT} (q : Qp) (v : o) : fractionalR o :=
+  (q, to_agree v).
+
+Lemma Some_valid:
+  forall M (A : cmraT) (x : cmra_car A),
+    (@uPred_cmra_valid (iResUR M) (optionR A) (@Some (cmra_car A) x)) -|-
+    (@uPred_cmra_valid (iResUR M) A x).
+Proof.
+  intros M A x.
+  rewrite (@uPred_primitive.option_validI (iResUR M) _ (Some x)). reflexivity.
+Qed.
+Lemma None_valid:
+  forall M (A : cmraT) (x : cmra_car A),
+    (@uPred_cmra_valid (iResUR M) (optionR A) None) -|- bi_pure True.
+Proof.
+  intros M A x.
+  rewrite (@uPred_primitive.option_validI (iResUR M) _ None). reflexivity.
+Qed.
+
+Lemma join_singleton_eq : forall `{Countable K, EqDecision K} {V : cmraT} (k : K) (v1 v2 : V),
+    {[ k := v1 ]} ⋅ {[ k := v2 ]} =@{gmap K V} {[ k := v1 ⋅ v2 ]}.
+Proof. intros. by apply (merge_singleton _ _ _ v1 v2). Qed.
+
+Lemma singleton_valid_norm :
+  ltac:(match type of @singleton_valid with
+        | ?T => let X := eval simpl in T in exact X
+        end).
+Proof. exact @singleton_valid. Defined.
+
+Lemma frac_op {A : ofeT} (l : A)  (p q : Qp) :
+  frac p l ⋅ frac q l ≡ frac (p + q) l.
+Proof. by rewrite -pair_op agree_idemp. Qed.
+
+
+(** soundness proof *)
+
+Module SimpleCPP
+(*  : CPP_LOGIC. (* Coq takes a long time checking this with the type ascription *) *).
+
+  Definition addr : Set := N.
+  Definition byte : Set := N.
+  Variant runtime_val : Set :=
+  | Rundef
+    (* ^ undefined value, semantically, it means "any value" *)
+  | Rval (_ : byte)
+    (* ^ machine level byte *)
+  | Rpointer_chunk (_ : ptr) (index : nat).
+    (* ^ you need the same pointer and consecutive integers to "have" a pointer.
+     *)
+
+  Class cppG' (Σ : gFunctors) : Type :=
+    { memG : inG Σ (gmapR addr (fractionalR (leibnizO runtime_val)))
+      (* ^ this represents the contents of physical memory *)
+    ; ghost_memG : inG Σ (gmapR ptr (fractionalR (leibnizO val)))
+      (* ^ this represents the contents of the C++ runtime that might
+         not be represented in physical memory, e.g. values stored in
+         registers or temporaries on the stack *)
+    ; localG : inG Σ (gmapUR region (gmapUR ident (exclR (leibnizO ptr))))
+      (* ^ this provides locations for local variables *)
+    ; mem_injG : inG Σ (gmapUR ptr (agreeR (leibnizO (option addr))))
+      (* ^ this carries the (compiler-supplied) mapping from C++ locations
+         (represented as pointers) to physical memory addresses. Locations that
+         are not stored in physical memory (e.g. because they are register
+         allocated) are mapped to [None] *)
+    ; codeG : inG Σ (gmapUR ptr (agreeR (leibnizO (Func + Method + Ctor + Dtor))))
+      (* ^ this carries the (compiler-supplied) mapping from C++ locations
+         to the code stored at that location *)
+    ; has_inv' :> invG Σ
+    ; has_cinv' :> cinvG Σ
+    }.
+
+  Definition cppG : gFunctors -> Type := cppG'.
+  Definition has_inv : forall Σ, cppG Σ -> invG Σ := @has_inv'.
+  Definition has_cinv : forall Σ, cppG Σ -> cinvG Σ := @has_cinv'.
+  Existing Class cppG.
+
+  Record cpp_ghost : Type :=
+    { heap_name : gname
+    ; ghost_heap_name : gname
+    ; local_name : gname
+    ; mem_inj_name : gname
+    ; code_name : gname
+    }.
+  Definition _cpp_ghost := cpp_ghost.
+
+  Class cpp_logic {thread_info : biIndex} : Type :=
+  { _Σ : gFunctors
+  ; _ghost : _cpp_ghost
+  ; has_cppG :> cppG _Σ }.
+  Arguments cpp_logic : clear implicits.
+  Coercion _Σ : cpp_logic >-> gFunctors.
+
+  Section with_cpp.
+    Context `{Σ : cpp_logic}.
+
+    Definition mpred := iProp Σ.
+    Definition mpredI : bi :=
+      {| bi_car := mpred
+       ; bi_ofe_mixin := (iPropI Σ).(bi_ofe_mixin)
+       ; bi_bi_mixin := (iPropI Σ).(bi_bi_mixin) |}.
+    (* todo: Fix the warning generated from this definition *)
+    Definition mpredSI : sbi :=
+      {| sbi_car := mpred
+       ; sbi_ofe_mixin := (iPropI Σ).(bi_ofe_mixin)
+       ; sbi_bi_mixin := (iPropI Σ).(bi_bi_mixin)
+       ; sbi_sbi_mixin := (iPropSI Σ).(sbi_sbi_mixin) |}.
+
+    Lemma singleton_valid_at_norm :
+      ∀ (K : Type) (EqDecision0 : EqDecision K) (H : Countable K) (A : cmraT) (i : K) (x : A),
+        ✓ ({[i := x]} : gmap K A) ⊣⊢@{mpredI} ✓ x.
+    Proof.
+      intros. simpl. rewrite gmap_validI.
+      split'.
+      - iIntros "X".
+        iDestruct ("X" $! i) as "X".
+        rewrite lookup_insert.
+        iStopProof.
+        clear.
+        rewrite Some_valid.
+        reflexivity.
+      - iIntros "X" (lll).
+        destruct (decide (i = lll)).
+        + subst. rewrite lookup_insert. rewrite Some_valid. iFrame.
+        + rewrite lookup_insert_ne; eauto.
+    Qed.
+
+    Definition Z_to_bytes (n : nat) (v : Z) : list runtime_val :=
+      let p := Z.modulo v (2 ^ n) in
+      Rval <$> List.rev ((fun i : nat => Z.to_N (Z.land 255 (Z.shiftr p (8 * i)))) <$> seq 0 n).
+
+    Definition size_to_bytes (s : types.size) : nat :=
+      match s with
+      | W8 => 1
+      | W16 => 2
+      | W32 => 4
+      | W64 => 8
+      | W128 => 16
+      end.
+    Definition POINTER_BYTES : nat := 8.
+
+    Definition aptr (p : ptr) : list runtime_val :=
+      List.map (Rpointer_chunk p) (seq 0 POINTER_BYTES).
+
+    Definition cptr (a : N) : list runtime_val :=
+      Z_to_bytes POINTER_BYTES (Z.of_N a).
+
+    Definition encodes (σ : genv) (t : type) (v : val) (vs : list runtime_val) : mpred.
+    refine
+      match erase_qualifiers t with
+      | Tint sz sgn
+      | Tchar sz sgn =>
+        match v with
+        | Vint v => [| vs = Z_to_bytes (size_to_bytes sz) v |]
+        | _ => lfalse
+        end
+      | Tmember_pointer _ _ =>
+        match v with
+        | Vint v =>
+          (* note: this is really an offset *)
+          [| vs = Z_to_bytes POINTER_BYTES v |]
+        | _ => lfalse
+        end
+
+      | Tbool =>
+        match v with
+        | Vint 0 => [| vs = Rval 0%N :: nil |]
+        | Vint 1 => [| vs = Rval 1%N :: nil |]
+        | _ => lfalse
+        end
+      | Tnullptr =>
+        [| vs = cptr 0 |]
+      | Tfloat _ => lfalse
+      | Tarch _ _ => lfalse
+      | Tpointer _ =>
+        match v with
+        | Vptr p =>
+          if decide (p = nullptr) then
+            [| vs = cptr 0 |]
+          else
+            Exists (l : option addr),
+              own _ghost.(mem_inj_name) {[ p := to_agree l ]} **
+              match l with
+              | None => [| vs = aptr p |]
+              | Some l => [| vs = cptr l |]
+              end
+        | _ => lfalse
+        end
+      | Tfunction _ _
+      | Treference _
+      | Trv_reference _ =>
+        match v with
+        | Vptr p =>
+          [| p <> nullptr |] **
+          Exists (l : option addr),
+            own _ghost.(mem_inj_name) {[ p := to_agree l ]} **
+            match l with
+            | None => [| vs = aptr p |]
+            | Some l => [| vs = cptr l |]
+            end
+        | _ => lfalse
+        end
+      | Tqualified _ _ => lfalse (* unreachable *)
+      | Tvoid
+      | Tarray _ _
+      | Tnamed _ => lfalse (* not directly encoded in memory *)
+      end.
+    all: try (unshelve eapply mem_injG; apply has_cppG).
+    all: refine _.
+    Defined.
+
+    Instance encodes_persistent : forall σ t v vs, Persistent (encodes σ t v vs).
+    Proof.
+      unfold encodes.
+      intros; destruct (erase_qualifiers t); intros;
+        destruct v; try refine _.
+      - destruct (decide (p = nullptr)); refine _.
+      - destruct z; refine _.
+        destruct p; refine _.
+    Qed.
+
+    Instance encodes_proper :
+      Proper (genv_leq ==> eq ==> eq ==> eq ==> lentails) encodes.
+    Proof.
+      do 6 red. intros; subst. reflexivity.
+    Qed.
+
+    Local Ltac go_encode X Y :=
+      let ll := fresh in
+      let rr := fresh in
+        iDestruct X as (ll) "[OL ZL]";
+        iDestruct Y as (rr) "[OR ZR]";
+        iDestruct (own_valid_2 with "OL OR") as X;
+        rewrite join_singleton_eq singleton_valid_at_norm
+                agree_validI agree_equivI;
+        iDestruct X as %[];
+        destruct ll; iDestruct "ZR" as %[]; iFrame.
+
+    Theorem encodes_consistent : forall σ t v a b,
+        encodes σ t v a ** encodes σ t v b |-- [| a = b |].
+    Proof.
+      unfold encodes.
+      intros; destruct (erase_qualifiers t); intros;
+        destruct v; try refine _.
+      all: try solve [ iIntros "[X Y]"; iDestruct "X" as %[]
+                     | iIntros "[X Y]"; iDestruct "Y" as %[]; iFrame ].
+      - destruct (decide (p = nullptr)).
+        + iIntros "[X Y]"; iDestruct "Y" as %[]; iFrame.
+        + iIntros "[X Y]".
+          go_encode "X" "Y".
+      - iIntros "[[_ X] [_ Y]]"; go_encode "X" "Y".
+      - iIntros "[[_ X] [_ Y]]"; go_encode "X" "Y".
+      - iIntros "[[_ X] [_ Y]]"; go_encode "X" "Y".
+      - destruct z;
+        try (iIntros "[X Y]"; iDestruct "Y" as %[]; iFrame).
+        destruct p; try (iIntros "[X Y]"; iDestruct "Y" as %[]; iFrame).
+    Qed.
+
+    Instance encodes_timeless : forall σ t v a, Timeless (encodes σ t v a).
+    Proof.
+      intros. unfold encodes. destruct (erase_qualifiers t); destruct v; refine _.
+      - destruct (decide (p = nullptr)); refine _.
+      - destruct z; refine _.
+        destruct p; refine _.
+    Qed.
+
+    Definition val_ (a : ptr) (v : val) (q : Qp) : mpred.
+    refine (
+      own _ghost.(ghost_heap_name) {[ a := frac (o:=leibnizO val) q v ]}).
+    apply (@ghost_memG Σ); apply has_cppG.
+    refine _.
+    Defined.
+
+    Instance: Fractional (val_ a rv).
+    Proof.
+      unfold val_. red.
+      intros.
+      etransitivity; [ | eapply own_op ].
+      eapply own_proper.
+      by rewrite op_singleton frac_op.
+    Qed.
+
+    Instance: AsFractional (val_ a rv q) (fun q => val_ a rv q) q.
+    Proof. constructor. reflexivity. refine _. Qed.
+
+    Instance: Timeless (val_ a rv q).
+    Proof. intros; refine _. Qed.
+
+
+    Definition byte_ (a : addr) (rv : runtime_val) (q : Qp) : mpred.
+    refine (
+      own _ghost.(heap_name) {[ a := frac (o:=leibnizO _) q rv ]}).
+    apply (@memG Σ); apply has_cppG.
+    refine _.
+    Defined.
+
+    Instance: Fractional (byte_ a rv).
+    Proof.
+      unfold byte_. red.
+      intros.
+      match goal with
+      | |- _ -|- @own ?S ?O ?Z ?G ?L ** own _ ?R =>
+        rewrite <- (@own_op S O Z G L R)
+      end.
+      eapply own_proper.
+      red. red. red. simpl. red. intros.
+      destruct (decide (a = i)); subst.
+      { rewrite lookup_op.
+        repeat rewrite lookup_insert.
+        rewrite -Some_op.
+        rewrite frac_op. reflexivity. }
+      { rewrite lookup_op.
+        repeat rewrite lookup_singleton_ne; eauto. }
+    Qed.
+
+    Instance: AsFractional (byte_ a rv q) (fun q => byte_ a rv q) q.
+    Proof. constructor. reflexivity. refine _. Qed.
+
+    Instance: Timeless (byte_ a rv q).
+    Proof. intros; refine _. Qed.
+
+    Definition bytes (a : addr) (vs : list runtime_val) (q : Qp) : mpred.
+    refine (
+      [∗list] ov ∈ zip (seq 0 (List.length vs)) vs,
+        (let '(o,rv) := ov in
+        byte_ (a+N.of_nat o)%N rv) q)%I.
+    Defined.
+
+    Instance: Timeless (bytes a rv q).
+    Proof. unfold bytes.
+           intros; refine _.
+           eapply big_sepL_timeless.
+           intros. destruct x.
+           refine _.
+    Qed.
+
+    Instance: Fractional (bytes a vs).
+    Proof. red. unfold bytes.
+           intros.
+           eapply fractional_big_sepL.
+           intros. destruct x. refine _.
+    Qed.
+
+    Instance: AsFractional (bytes a vs q) (bytes a vs) q.
+    Proof. constructor; refine _. reflexivity. Qed.
+
+
+    (* heap points to *)
+    Definition tptsto {σ:genv} (t : type) (q : Qp) (p : ptr) (v : val) : mpred.
+    Proof.
+      refine (Exists (a : option addr),
+              [| has_type v t |] **
+              own _ghost.(mem_inj_name) {[ p := to_agree a ]} **
+              match a with
+              | Some a =>
+                Exists vs,
+                encodes σ t v vs ** bytes a vs q
+              | None => val_ p v q
+              end).
+      1: apply (@mem_injG Σ); apply has_cppG.
+      refine _.
+    Defined.
+
+    Theorem tptsto_proper_entails :
+      Proper (genv_leq ==> eq ==> eq ==> eq ==> eq ==> lentails) (@tptsto).
+    Proof.
+      do 6 red; intros; subst.
+      unfold tptsto.
+      iIntros "H".
+      iDestruct "H" as (a) "[#De [#Mi Lo]]".
+      iExists (a).
+      iFrame "#".
+      iFrame.
+    Qed.
+    Theorem tptsto_proper_equiv :
+      Proper (genv_eq ==> eq ==> eq ==> eq ==> eq ==> lequiv) (@tptsto).
+    Proof.
+      do 6 red; intros. split';
+       eapply tptsto_proper_entails; eauto; apply H.
+    Qed.
+
+    Theorem tptsto_fractional :
+      forall {σ} ty p v, Fractional (λ q, @tptsto σ ty q p v).
+    Proof.
+      red. intros. unfold tptsto.
+      iSplit.
+      - iIntros "H".
+        iDestruct "H" as (a) "[#De [#Mi By]]".
+        destruct a.
+        + iDestruct "By" as (vs) "[#En By]".
+          rewrite fractional.
+          iDestruct "By" as "[L R]".
+          iSplitL "L".
+          * iExists (Some a); iFrame; iFrame "#". iExists vs. iFrame "#". eauto.
+          * iExists (Some a); iFrame; iFrame "#". iExists vs. iFrame "#". eauto.
+        + rewrite fractional.
+          iDestruct "By" as "[L R]".
+          iSplitL "L".
+          * iExists None; iFrame; iFrame "#".
+          * iExists None; iFrame; iFrame "#".
+      - iIntros "[H1 H2]".
+        iDestruct "H1" as (a) "[#De1 [#Mi1 By1]]".
+        iDestruct "H2" as (a2) "[#De2 [#Mi2 By2]]".
+        iExists a; iFrame "#".
+        iDestruct (own_valid_2 with "Mi1 Mi2") as "X".
+        rewrite join_singleton_eq.
+        rewrite singleton_valid_at_norm.
+        rewrite agree_validI.
+        rewrite agree_equivI.
+        iDestruct "X" as %[].
+        destruct a.
+        + iDestruct "By1" as (vs) "[#En1 By1]".
+          iDestruct "By2" as (vs2) "[#En2 By2]".
+          iDestruct (encodes_consistent with "[En1 En2]") as "Z".
+          { iSplit. iApply "En1". iApply "En2". }
+          iDestruct "Z" as %[].
+          iExists vs; iFrame "#".
+          rewrite fractional. iFrame.
+        + rewrite fractional. iFrame.
+    Qed.
+    Theorem tptsto_as_fractional :
+      forall {σ} ty q p v, AsFractional (@tptsto σ ty q p v) (λ q, @tptsto σ ty q p v)%I q.
+    Proof.
+      intros. constructor. reflexivity.
+      apply tptsto_fractional.
+    Qed.
+
+    Theorem tptsto_timeless :
+      forall {σ} ty q p v, Timeless (@tptsto σ ty q p v).
+    Proof.
+      intros. unfold tptsto. red.
+      iIntros "H".
+      iDestruct "H" as (a) "[#H [X Y]]".
+      iExists a.
+      repeat rewrite timeless.
+      iSplit; iFrame "#".
+      iSplit; iFrame.
+    Qed.
+
+    Theorem tptsto_has_type : forall σ t q p v,
+        @tptsto σ t q p v |-- @tptsto σ t q p v ** [| has_type v t |].
+    Proof.
+      unfold tptsto.
+      intros.
+      iIntros "H".
+      iDestruct "H" as (a) "[#H X]".
+      iFrame "#".
+      iExists a. iFrame.
+    Qed.
+
+    (* this is like a "points to" where the location is (region * ident).
+     *)
+    Definition local_addr (ρ : region) (i : ident) (p : ptr) : mpred.
+      refine (own _ghost.(local_name) {[ ρ := {[ i := Excl p ]} ]}).
+      apply (@localG Σ); apply has_cppG.
+      all: refine _.
+    Defined.
+
+    (** the pointer points to the code
+
+      note that in the presence of code-loading, function calls will
+      require an extra side-condition that the code is loaded.
+     *)
+    Definition code_at (f : Func) (p : ptr) : mpred.
+    refine (own _ghost.(code_name) {[ p := to_agree (inl (inl (inl f))) ]}).
+    apply (@codeG Σ); apply has_cppG.
+    all: refine _.
+    Defined.
+
+    Definition method_at (m : Method) (p : ptr) : mpred.
+    refine (own _ghost.(code_name) {[ p := to_agree (inl (inl (inr m))) ]}).
+    apply (@codeG Σ); apply has_cppG.
+    all: refine _.
+    Defined.
+
+    Definition ctor_at (c : Ctor) (p : ptr) : mpred.
+    refine (own _ghost.(code_name) {[ p := to_agree (inl (inr c)) ]}).
+    apply (@codeG Σ); apply has_cppG.
+    all: refine _.
+    Defined.
+
+    Definition dtor_at (d : Dtor) (p : ptr) : mpred.
+    refine (own _ghost.(code_name) {[ p := to_agree (inr d) ]}).
+    apply (@codeG Σ); apply has_cppG.
+    all: refine _.
+    Defined.
+
+    Theorem code_at_persistent : forall f p, Persistent (@code_at f p).
+    Proof. red. intros. iIntros "#X". iFrame "#". Qed.
+    Theorem code_at_affine : forall f p, Affine (@code_at f p).
+    Proof. red. intros. eauto. Qed.
+
+    Theorem method_at_persistent : forall f p, Persistent (@method_at f p).
+    Proof. red. intros. iIntros "#X". iFrame "#". Qed.
+    Theorem method_at_affine : forall f p, Affine (@method_at f p).
+    Proof. red. intros. eauto. Qed.
+
+    Theorem ctor_at_persistent : forall f p, Persistent (@ctor_at f p).
+    Proof. red. intros. iIntros "#X". iFrame "#". Qed.
+    Theorem ctor_at_affine : forall f p, Affine (@ctor_at f p).
+    Proof. red. intros. eauto. Qed.
+
+    Theorem dtor_at_persistent : forall f p, Persistent (@dtor_at f p).
+    Proof. red. intros. iIntros "#X". iFrame "#". Qed.
+    Theorem dtor_at_affine : forall f p, Affine (@dtor_at f p).
+    Proof. red. intros. eauto. Qed.
+
+  End with_cpp.
+
+End SimpleCPP.
